RocqOfRust/revm/revm_interpreter/instructions/simulate/memory/mcopy.v
@@ -2,8 +2,10 @@ Require Import simulate.RocqOfRust.
 Require Import alloy_primitives.links.aliases.
 Require Import core.links.array.
 Require Import core.ops.simulate.deref.
+Require Import core.simulate.cmp.
 Require Import core.simulate.option.
 Require Import revm.revm_context_interface.links.host.
+Require Import revm.revm_interpreter.gas.simulate.calc.
 Require Import revm.revm_interpreter.gas.simulate.constants.
 Require Import revm.revm_interpreter.instructions.links.memory.mcopy.
 Require Import revm.revm_interpreter.instructions.simulate.macros.
@@ -27,16 +29,14 @@ Definition mcopy
     Interpreter.t WIRE WIRE_types :=
   check_macro interpreter SpecId.CANCUN id (fun interpreter =>
   popn_macro interpreter {| Integer.value := 3 |} id (fun arr interpreter =>
-  let '⟬ dst_u256; src_u256; len_u256 ⟭ := arr.(array.value) in
-  as_usize_or_fail_ret_macro interpreter len_u256 None id (fun len interpreter =>
+  let '⟬ dst; src; len ⟭ := arr.(array.value) in
+  as_usize_or_fail_ret_macro interpreter len None id (fun len interpreter =>
+  gas_or_fail_macro interpreter (calc.copy_cost_verylow len) id (fun interpreter =>
   if i[len] =? 0 then
     interpreter
   else
-    as_usize_or_fail_ret_macro interpreter dst_u256 None id (fun dst interpreter =>
-    as_usize_or_fail_ret_macro interpreter src_u256 None id (fun src interpreter =>
-    let words_num := num_words len in
-    let copy_cost : u64 := {| Integer.value := i[constants.VERYLOW] + i[words_num] * i[constants.COPY] |} in
-    gas_macro interpreter copy_cost id (fun interpreter =>
+    as_usize_or_fail_ret_macro interpreter dst None id (fun dst interpreter =>
+    as_usize_or_fail_ret_macro interpreter src None id (fun src interpreter =>
     let max_offset : usize := {| Integer.value := Z.max i[dst] i[src] |} in
     resize_memory_macro interpreter max_offset len id (fun interpreter =>
     let memory :=
@@ -79,11 +79,34 @@ Proof.
     destruct array as [[dst_u256 [src_u256 [len_u256 []]]]]
   end.
   as_usize_or_fail_macro_eq InterpreterTypesEq.
-  resize_memory_macro_eq InterpreterTypesEq.
+  s. {
+    apply calc.copy_cost_verylow_eq.
+  }
+  unfold gas_macro.
   s. {
     apply InterpreterTypesEq.
   }
   s. {
-    apply InterpreterTypesEq.
+    apply Impl_Gas.record_cost_eq.
   }
+  destruct Impl_Gas.record_cost. 2: {
+    s. {
+      apply InterpreterTypesEq.
+    }
+    s.
+  }
+  s.
+  destruct (_ =? 0); [s|].
+  as_usize_or_fail_macro_eq InterpreterTypesEq.
+  as_usize_or_fail_macro_eq InterpreterTypesEq.
+  s. {
+    (* max *)
+    s. {
+      s. {
+        s. {
+          s. {
+            s_apply Impl_Ord_for_usize.cmp_eq.
+          }
+          s.
+        }
 Admitted.
